1. $\sum_{n=0}^{\infty}{\frac{x^{2^n}}{1-x^{2^{n+1}}}}$
   $\text{è§£}:\sum_{n=0}^{\infty}{\frac{x^{2^n}}{1-x^{2^{n+1}}}}=\sum_{n=0}^{\infty}{\left( \frac{1}{1-x^{2^n}}-\frac{1}{1-x^{2^{n+1}}} \right)}$
   $=\frac{1}{1-x}
   \\$
2. $\sum_{n=1}^{\infty}{\mathrm{arc}\tan \left( \frac{1}{2k^2} \right)}=\sum_{n=1}^{\infty}{\left( \mathrm{arc}\tan \left( \frac{\left( 2k+1 \right) -\left( 2k-1 \right)}{1+\left( 2k-1 \right) \left( 2k+1 \right)} \right) \right)}
   \\$
   $=\sum_{n=1}^{\infty}{\mathrm{arc}\tan \left( 2k+1 \right) -\mathrm{arc}\tan \left( 2k-1 \right)}
   \\
   =\frac{\pi}{2}-\frac{\pi}{4}
   \\
   =\frac{\pi}{4}
   \\$
3. $\sum_{k=2}^{\infty}{\mathrm{arc}\tan \left( \frac{2}{4k^2-4k+1} \right)}=\sum_{k=2}^{\infty}{\mathrm{arc}\tan \left( \frac{2k-\left( 2k-2 \right)}{2k\left( 2k-2 \right) +1} \right)}
   \\$
   $=\sum_{k=2}^{\infty}{\left( \mathrm{arc}\tan \left( 2k \right) -\mathrm{arc}\tan \left( 2k-2 \right) \right)}
   \\
   =\frac{\pi}{2}-\mathrm{arc}\tan \left( 2 \right) 
   \\$